allocate output buffer ourselves

steel/Zeta.Steel.ExternalPtr.fst
@@ -16,37 +16,16 @@ val enclave_api_validate (x:A.array U8.t) (n: U32.t) : Pure bool
   (requires True)
   (ensures (fun b -> b == true ==> U32.v n == A.length x))
 
-let valid_input = enclave_api_validate
-
 let copy_extern_input_ptr
-  e n
+  e n a
 =
-  let res = A.alloc 0uy n in
-  rewrite (has_extern_input_ptr e n) (has_extern_input_ptr0 e n);
-  let _ = gen_elim () in
-  A.memcpy e res n;
-  rewrite (has_extern_input_ptr0 e n) (has_extern_input_ptr e n);
-  return res
-
-let extern_output_ptr = A.array U8.t
-
-let gtake p = p
-
-let valid_output = enclave_api_validate
-
-let take x n = x
-
-assume
-val enclave_api_check_input_output_disjoint
-  (input: extern_input_ptr)
-  (input_len: U32.t)
-  (output: extern_output_ptr)
-  (output_len: U32.t)
-  (output_contents: Ghost.erased (Seq.seq U8.t))
-: ST bool
-    (has_extern_input_ptr input input_len `sl_and` A.pts_to (gtake output) full_perm output_contents)
-    (fun b -> check_disjoint_post b (has_extern_input_ptr input input_len) (A.pts_to (gtake output) full_perm output_contents))
-    (valid_input input input_len /\ valid_output output output_len)
-    (fun _ -> True)
-
-let check_input_output_disjoint = enclave_api_check_input_output_disjoint
+  if enclave_api_validate e n
+  then begin
+    rewrite (has_extern_input_ptr e n) (has_extern_input_ptr0 e n);
+    let _ = gen_elim () in
+    A.memcpy e a n;
+    rewrite (has_extern_input_ptr0 e n) (has_extern_input_ptr e n);
+    return true
+  end else begin
+    return false
+  end
