steel/Zeta.Steel.SafeMain.fst
@@ -23,7 +23,7 @@ let gather ts ts' =
   let _ = gen_elim () in
   rewrite (handle_pts_to ts') (handle_pts_to0 ts');
   let _ = gen_elim () in
-  gather_body _;
+  gather_body handle.state;
   rewrite (handle_pts_to0 ts) (handle_pts_to ts)
 
 let share
@@ -112,18 +112,15 @@ let verify_log_some_concl
                (input: EXT.extern_input_ptr)
                (out_len: U32.t)
                (#out_bytes:Ghost.erased AT.bytes)
-               (output: EXT.extern_output_ptr)
-               (sq: squash (check_verify_input tid len input out_len output))
+               (sq: squash (check_verify_input tid len))
                (input': U.larray U8.t len)
                (output' : U.larray U8.t out_len)
                (entries: Ghost.erased AEH.log)
   (p1: perm)
   (v: option (M.verify_result len))
-: STGhost unit opened
+: STGhostT unit opened
     (R.pts_to handle.state.state p1 handle.state.tl_state `star` M.verify_post handle.state.tl_state tid entries log_perm log_bytes len input' out_len out_bytes output' v `star` EXT.has_extern_input_ptr input len)
-    (fun _ -> verify_post tid len input out_len out_bytes output v `star` A.pts_to input' log_perm log_bytes)
-    (output' == EXT.gtake output)
-    (fun _ -> True)
+    (fun _ -> verify_post tid len input v `star` A.pts_to input' log_perm log_bytes `star` (exists_ (A.pts_to output' full_perm)))
 = if (Some? v && V.Verify_success? (Some?.v v))
   then begin
     let Some (V.Verify_success read wrote) = v in
@@ -137,92 +134,107 @@ let verify_log_some_concl
     rewrite (handle_pts_to_body0 handle.state) (handle_pts_to_body handle.state);
     rewrite (M.log_of_tid_gen _ _ _) emp;
     rewrite (handle_pts_to0 handle.state.tl_state) (handle_pts_to handle.state.tl_state);
-    let out_bytes' = vpattern_replace_erased (A.pts_to output' _) in
-    vpattern_rewrite #_ #_ #output' (fun output -> A.pts_to output _ _) (EXT.gtake output);
     rewrite
-      (verify_post_some_m_success tid len input out_len out_bytes output v () handle.state.tl_state read wrote)
-      (verify_post_some_m tid len input out_len out_bytes output v handle.state.tl_state);
+      (verify_post_some_m_success tid len input v () handle.state.tl_state read wrote)
+      (verify_post_some_m tid len input v handle.state.tl_state);
     rewrite
-      (verify_post_some tid len input out_len out_bytes output _)
-      (verify_post tid len input out_len out_bytes output v)
+      (verify_post_some tid len input _)
+      (verify_post tid len input v)
   end else begin
     m_verify_post_failure_eq handle.state.tl_state tid entries log_perm log_bytes len input' out_len out_bytes output' v;
     let _ = gen_elim () in
     rewrite (handle_pts_to_body0 handle.state) (handle_pts_to_body handle.state);
     rewrite (handle_pts_to0 handle.state.tl_state) (handle_pts_to handle.state.tl_state);
-    vpattern_rewrite #_ #_ #output' (fun output -> A.pts_to output _ _) (EXT.gtake output);
-    EXT.star_sl_and (EXT.has_extern_input_ptr _ _) (A.pts_to (EXT.gtake output) _ _);
     rewrite
-      (verify_post_some_m_failure len input output)
-      (verify_post_some_m tid len input out_len out_bytes output v handle.state.tl_state);
+      (verify_post_some_m_failure len input)
+      (verify_post_some_m tid len input v handle.state.tl_state);
     rewrite
-      (verify_post_some tid len input out_len out_bytes output _)
-      (verify_post tid len input out_len out_bytes output v)
+      (verify_post_some tid len input _)
+      (verify_post tid len input v)
   end
 
 let verify_log_some
                (tid:U16.t)
                (len: U32.t)
                (input: EXT.extern_input_ptr)
+               (input': U.larray U8.t len)
                (out_len: U32.t)
-               (#out_bytes:Ghost.erased AT.bytes)
-               (output: EXT.extern_output_ptr)
-  : ST (option (v:V.verify_result { V.verify_result_complete len v }))
+               (output': A.array U8.t)
+  : ST (option (M.verify_result len))
     (handle_pts_to_body handle.state `star`
       EXT.has_extern_input_ptr input len `star`
-     A.pts_to (EXT.gtake output) full_perm out_bytes
+      (exists_ (A.pts_to input' full_perm)) `star`
+      (exists_ (A.pts_to output' full_perm))
     )
-    (fun res -> verify_post tid len input out_len out_bytes output res)
-    (check_verify_input tid len input out_len output)
+    (fun res -> verify_post tid len input res)
+    (check_verify_input tid len /\
+      A.adjacent input' output' /\
+      A.is_full_array (A.merge input' output') /\
+      U32.v out_len == A.length output'
+    )
     (fun _ -> True)
 =
-  let input' = EXT.copy_extern_input_ptr input len in
   rewrite (handle_pts_to_body handle.state) (handle_pts_to_body0 handle.state);
   let _ = gen_elim () in
   rewrite emp (M.log_of_tid_gen handle.state.tl_state tid Seq.empty);
-  let output' = EXT.take output out_len in
-  vpattern_rewrite (fun a -> A.pts_to a full_perm out_bytes) output';
   let v = M.verify_log _ tid len input' out_len output' in
-  let _ = verify_log_some_concl tid len input out_len output () input' output' _ _ v in
-  A.free input';
+  let _ = verify_log_some_concl tid len input out_len () input' output' _ _ v in
+  let _ = gen_elim () in
+  let a = A.join input' output' in
+  A.free a;
   return v
 
+inline_for_extraction
+noextract
+let steel_ifthenelse
+  (#t: Type)
+  (#vpre: vprop)
+  (#vpost: (t -> vprop))
+  (b: bool)
+  (ttrue: (squash (b == true) -> STT t vpre vpost))
+  (tfalse: (squash (b == false) -> STT t vpre vpost))
+: STF t vpre vpost True (fun _ -> True)
+= if b then ttrue () else tfalse ()
+
 let verify_log
-  tid len input out_len #out_bytes output
+  tid len input
 =
   let t = handle.state.tl_state in
   handle_pts_to_body_intro ();
-  if not (check_verify_input tid len input out_len output) returns STT (option (M.verify_result len))
-    (handle_pts_to_body handle.state `star` verify_pre len input out_bytes output)
-    (fun res -> verify_post tid len input out_len out_bytes output res)
-  then begin
+  steel_ifthenelse
+    (not (check_verify_input tid len))
+  (fun _ ->
     noop ();
     rewrite (handle_pts_to0 t) (handle_pts_to t);
-    rewrite (verify_post_some_m_failure len input output) (verify_post_some_m tid len input out_len out_bytes output None t);
-    rewrite (verify_post_some tid len input out_len out_bytes output None)
-      (verify_post tid len input out_len out_bytes output None);
+    rewrite (verify_post_some_m_failure len input) (verify_post_some_m tid len input None t);
+    rewrite (verify_post_some tid len input None)
+      (verify_post tid len input None);
     return None
-  end else
-  begin
-    let check_disjoint = EXT.check_input_output_disjoint input len output out_len _ in
-    if check_disjoint
-    then begin
-      rewrite
-        (EXT.check_disjoint_post _ _ _)
-        (EXT.has_extern_input_ptr input len `star`
-          A.pts_to (EXT.gtake output) full_perm out_bytes);
-        verify_log_some tid len input out_len output
-    end else begin
-      rewrite
-        (EXT.check_disjoint_post _ _ _)
-        (verify_pre len input out_bytes output);
+  )
+  (fun _ ->
+    let a = A.alloc 0uy (len `U32.add` 1ul) in
+    A.ghost_split a len;
+    let input' = A.split_l a len in
+    let output' = A.split_r a len in
+    vpattern_rewrite #_ #_ #(A.split_l _ _) (fun a -> A.pts_to a _ _) input';
+    vpattern_rewrite #_ #_ #(A.split_r _ _) (fun a -> A.pts_to a _ _) output';
+    let check_copy = EXT.copy_extern_input_ptr input len input' in
+    let _ = gen_elim () in
+    steel_ifthenelse check_copy
+    (fun _ ->
+      noop ();
+      verify_log_some tid len input input' 1ul output'
+    )
+    (fun _ ->
+      let a = A.join input' output' in
+      A.free a;
       rewrite (handle_pts_to0 t) (handle_pts_to t);
-      rewrite (verify_post_some_m_failure len input output) (verify_post_some_m tid len input out_len out_bytes output None t);
-      rewrite (verify_post_some tid len input out_len out_bytes output None)
-        (verify_post tid len input out_len out_bytes output None);
+      rewrite (verify_post_some_m_failure len input) (verify_post_some_m tid len input None t);
+      rewrite (verify_post_some tid len input None)
+        (verify_post tid len input None);
       return None
-    end
-  end
+    )
+  )
 
 let max_certified_epoch
   ()
