steel/Zeta.Steel.ExternalPtr.fsti
@@ -1,5 +1,4 @@
 module Zeta.Steel.ExternalPtr
-include Zeta.Steel.ExternalPtr.SLAnd
 
 // DO NOT FRIEND this module!
 
@@ -15,48 +14,12 @@ val extern_input_ptr : Type0
 val has_extern_input_ptr (e: extern_input_ptr) (n: U32.t) : vprop
 
 inline_for_extraction
-val valid_input (p: extern_input_ptr) (n: U32.t) : Tot bool
-
-inline_for_extraction
 val copy_extern_input_ptr
   (e: extern_input_ptr)
   (n: U32.t)
-: ST (A.array U8.t)
-    (has_extern_input_ptr e n)
-    (fun res -> has_extern_input_ptr e n `star` exists_ (fun contents -> A.pts_to res full_perm contents))
-    (valid_input e n)
-    (fun res -> A.is_full_array res /\ A.length res == U32.v n)
-
-inline_for_extraction
-val extern_output_ptr: Type0
-
-val gtake (p: extern_output_ptr) : GTot (A.array U8.t)
-
-inline_for_extraction
-val valid_output (p: extern_output_ptr) (n: U32.t) : Pure bool
-  (requires True)
-  (ensures (fun b -> b == true ==> U32.v n == A.length (gtake p)))
-
-inline_for_extraction
-val take (p: extern_output_ptr) (n: Ghost.erased U32.t) : Pure (A.array U8.t)
-  (requires (valid_output p n))
-  (ensures (fun y -> y == gtake p))
-
-let check_disjoint_post
-  (b: bool)
-  (p1 p2: vprop)
-: vprop
-= p1 `(if b then star else sl_and)` p2
-
-inline_for_extraction
-val check_input_output_disjoint
-  (input: extern_input_ptr)
-  (input_len: U32.t)
-  (output: extern_output_ptr)
-  (output_len: U32.t)
-  (output_contents: Ghost.erased (Seq.seq U8.t))
+  (a: A.array U8.t)
 : ST bool
-    (has_extern_input_ptr input input_len `sl_and` A.pts_to (gtake output) full_perm output_contents)
-    (fun b -> check_disjoint_post b (has_extern_input_ptr input input_len) (A.pts_to (gtake output) full_perm output_contents))
-    (valid_input input input_len /\ valid_output output output_len)
+    (has_extern_input_ptr e n `star` exists_ (fun contents -> A.pts_to a full_perm contents))
+    (fun _ -> has_extern_input_ptr e n `star` exists_ (fun contents -> A.pts_to a full_perm contents))
+    (A.length a == U32.v n)
     (fun _ -> True)
